p256: wip: use generic bignum for finv and fsqrt

code/ecdsap256/Hacl.Impl.P256.Core.fst
@@ -1,11 +1,9 @@
 module Hacl.Impl.P256.Core
 
+open FStar.Mul
 open FStar.HyperStack.All
 open FStar.HyperStack
 module ST = FStar.HyperStack.ST
-
-open FStar.Mul
-open FStar.Math.Lemmas
 
 open Lib.IntTypes
 open Lib.Buffer
@@ -17,15 +15,15 @@ open Hacl.Impl.P256.Field
 open Spec.P256.MontgomeryMultiplication
 friend Spec.P256.MontgomeryMultiplication
 
-#set-options "--z3rlimit 100 --fuel 0 --ifuel 0"
+#set-options "--z3rlimit 50 --fuel 0 --ifuel 0"
 
-let toDomain value result =
-  push_frame();
-    let multBuffer = create (size 8) (u64 0) in
-    bn_lshift256 value multBuffer;
-    solinas_reduction_impl multBuffer result;
+let toDomain f res =
+  push_frame ();
+  let multBuffer = create (size 8) (u64 0) in
+  bn_lshift256 f multBuffer;
+  solinas_reduction_impl multBuffer res;
   pop_frame()
 
 
-let fromDomain f result =
-  montgomery_multiplication_buffer_by_one f result
+let fromDomain f res =
+  montgomery_multiplication_buffer_by_one f res
