code/ecdsap256/Hacl.Impl.P256.Finv.fsti
@@ -9,26 +9,25 @@ open Lib.IntTypes
 open Lib.Buffer
 
 open Spec.P256
-open Spec.P256.Constants
-open Spec.P256.Lemmas
 open Spec.P256.MontgomeryMultiplication
-
 open Hacl.Spec.P256.Felem
+
+module M = Lib.NatMod
+module S = Spec.P256.Constants
 
 #set-options "--z3rlimit 30 --fuel 0 --ifuel 0"
 
-val finv: a:felem -> res:felem -> tmp:lbuffer uint64 (size 20) -> Stack unit
+val finv: a:felem -> res:felem -> Stack unit
   (requires fun h ->
-    live h a /\ live h tmp /\ live h res /\
-    disjoint tmp res /\ disjoint a tmp /\
-    as_nat h a < prime256)
-  (ensures fun h0 _ h1 -> modifies (loc res |+| loc tmp) h0 h1 /\
-    as_nat h1 res = toDomain_ ((pow (fromDomain_ (as_nat h0 a)) (prime256 - 2)) % prime256))
+    live h a /\ live h res /\ disjoint a res /\
+    as_nat h a < S.prime256)
+  (ensures fun h0 _ h1 -> modifies (loc res) h0 h1 /\
+    as_nat h1 res < S.prime256 /\
+    as_nat h1 res = toDomain_ (S.finv (fromDomain_ (as_nat h0 a))))
 
 
 val fsqrt: a:felem -> res:felem -> Stack unit
-  (requires fun h -> live h a /\ live h res /\ as_nat h a < prime)
-  (ensures fun h0 _ h1 -> modifies (loc a |+| loc res) h0 h1 /\
-    as_nat h1 res < prime /\
-    fromDomain_ (as_nat h1 res) = sq_root_spec (fromDomain_ (as_nat h0 a)) /\
-    fromDomain_ (as_nat h1 res) = pow (fromDomain_ (as_nat h0 a)) ((prime256 + 1) / 4) % prime256)
+  (requires fun h -> live h a /\ live h res /\ as_nat h a < S.prime256)
+  (ensures fun h0 _ h1 -> modifies (loc res) h0 h1 /\
+    as_nat h1 res < S.prime256 /\
+    as_nat h1 res = toDomain_ (S.fsqrt (fromDomain_ (as_nat h0 a))))
