specs/ecdsap256/Spec.P256.MontgomeryMultiplication.fsti
@@ -78,4 +78,3 @@ val _pow_step: k:lseq uint8 32 -> i:nat{i < 256} -> before:tuple2 nat_prime nat_
 
 val pow_spec: k:lseq uint8 32 -> a:nat_prime -> Tot (r: nat_prime {r = pow a (Lib.ByteSequence.nat_from_bytes_le k) % prime256})
 
-val sq_root_spec: a: nat_prime -> Tot (r: nat_prime {r = pow a ((prime256 + 1) / 4) % prime256})
